src/drf/SimWhole.v
@@ -1,0 +1,76 @@
+Require Import Program.
+Require Import sflib.
+Require Import paco.
+
+Require Import Axioms.
+Require Import Basic.
+Require Import Event.
+Require Import Language.
+Require Import View.
+Require Import Cell.
+Require Import Memory.
+Require Import TView.
+Require Import Thread.
+Require Import Configuration.
+
+Require Import SimMemory.
+Require Import SimPromises.
+Require Import Behavior.
+
+Set Implicit Arguments.
+
+
+Section SimWhole.
+  Variable (step_src step_tgt: forall (e:option Event.t) (tid:Ident.t) (c1 c2:Configuration.t), Prop).
+
+  Definition SIM_WHOLE := forall (c1_src c1_tgt:Configuration.t), Prop.
+
+  Inductive _sim_whole
+            (sim_whole: SIM_WHOLE)
+            (c1_src c1_tgt:Configuration.t): Prop :=
+  | _sim_whole_intro
+      (TERMINAL:
+         forall (TERMINAL_TGT: Threads.is_terminal c1_tgt.(Configuration.threads)),
+         exists c2_src,
+           <<STEPS: rtc (union (step_src None)) c1_src c2_src>> /\
+           <<TERMINAL_SRC: Threads.is_terminal c2_src.(Configuration.threads)>>)
+      (STEP:
+         forall e tid_tgt c3_tgt
+           (STEP_TGT: step_tgt e tid_tgt c1_tgt c3_tgt),
+         exists tid_src c2_src c3_src,
+           <<STEPS_SRC: rtc (union (step_src None)) c1_src c2_src>> /\
+           <<STEP_SRC: opt step_src e tid_src c2_src c3_src>> /\
+           <<SIM: sim_whole c3_src c3_tgt>>)
+  .
+
+  Lemma _sim_whole_mon: monotone2 _sim_whole.
+  Proof.
+    ii. inv IN. econs; eauto. i.
+    exploit STEP; eauto. i. des.
+    esplits; eauto.
+  Qed.
+  Hint Resolve _sim_whole_mon: paco.
+
+  Definition sim_whole: SIM_WHOLE := paco2 _sim_whole bot2.
+End SimWhole.
+Hint Resolve _sim_whole_mon: paco.
+
+
+Lemma sim_whole_adequacy
+      step_src step_tgt
+      c_src c_tgt
+      (SIM: sim_whole step_src step_tgt c_src c_tgt):
+  behaviors step_tgt c_tgt <1= behaviors step_src c_src.
+Proof.
+  s. i.
+  revert c_src SIM.
+  dependent induction PR; i.
+  - punfold SIM. inv SIM. exploit TERMINAL0; eauto. i. des.
+    eapply rtc_tau_step_behavior; eauto. econs 1. eauto.
+  - punfold SIM. inv SIM. exploit STEP0; eauto. i. des. inv SIM; ss.
+    eapply rtc_tau_step_behavior; eauto.
+    inv STEP_SRC. econs 2; eauto.
+  - punfold SIM. inv SIM. exploit STEP0; eauto. i. des. inv SIM; ss.
+    eapply rtc_tau_step_behavior; eauto.
+    inv STEP_SRC; eauto. econs 3; eauto.
+Qed.
